Rename SpillSoundFive -> SpillSoundSeven, Add proof for spill_sound -> spill_sound7

theories/Spilling/SpillSoundSeven.v
@@ -3,7 +3,10 @@ Require Import IL Annotation AnnP InRel.
 Require Import LabelsDefined SpillSound SpillUtil.
 
 
-Inductive spill_sound (k:nat) :
+(** * Correctness Predicate with 7 rules *)
+
+
+Inductive spill_sound7 (k:nat) :
   (list params)
   -> (list (⦃var⦄ * ⦃var⦄))
   -> (⦃var⦄ * ⦃var⦄)
@@ -21,11 +24,11 @@ Inductive spill_sound (k:nat) :
       (sl : spilling)
       (Sp_empty : Sp [=] ∅)
       (L_empty : L [=] ∅)
-      (spill_sub : spill_sound k ZL Λ ({x;R\Kx},M) s sl)
+      (spill_sub : spill_sound7 k ZL Λ ({x;R\Kx},M) s sl)
       (kgt0: k > 0)
       (card : cardinal {x; R \ Kx } <= k)
       (inR : Exp.freeVars e ⊆ R)
-      : spill_sound k ZL Λ (R,M) (stmtLet x e s) (ann1 (Sp,L,nil) sl)
+      : spill_sound7 k ZL Λ (R,M) (stmtLet x e s) (ann1 (Sp,L,nil) sl)
   | SpillReturn
       (ZL : list (params))
       (Λ : list (⦃var⦄ * ⦃var⦄))
@@ -34,7 +37,7 @@ Inductive spill_sound (k:nat) :
       (Sp_empty : Sp [=] ∅)
       (L_empty : L [=] ∅)
       (inVar : Op.freeVars e ⊆ R)
-      : spill_sound k ZL Λ (R,M) (stmtReturn e) (ann0 (Sp,L,nil))
+      : spill_sound7 k ZL Λ (R,M) (stmtReturn e) (ann0 (Sp,L,nil))
   | SpillIf
       (ZL : list (params))
       (Λ : list (⦃var⦄ * ⦃var⦄))
@@ -45,9 +48,9 @@ Inductive spill_sound (k:nat) :
       (Sp_empty : Sp [=] ∅)
       (L_empty : L [=] ∅)
       (inVar : Op.freeVars e ⊆ R)
-      (spill_s : spill_sound k ZL Λ (R,M) s sl_s)
-      (spill_t : spill_sound k ZL Λ (R,M) t sl_t)
-    : spill_sound k ZL Λ (R,M) (stmtIf e s t) (ann2 (Sp,L,nil) sl_s sl_t)
+      (spill_s : spill_sound7 k ZL Λ (R,M) s sl_s)
+      (spill_t : spill_sound7 k ZL Λ (R,M) t sl_t)
+    : spill_sound7 k ZL Λ (R,M) (stmtIf e s t) (ann2 (Sp,L,nil) sl_s sl_t)
   | SpillApp
       (ZL : list params)
       (Λ : list (⦃var⦄ * ⦃var⦄))
@@ -63,7 +66,7 @@ Inductive spill_sound (k:nat) :
       (Mf_sub : M_f \ of_list Z ⊆ M)
       (inVar : list_union (Op.freeVars ⊝ Y) ⊆ R ∪ M')
       (M_sub : M' ⊆ M)
-      : spill_sound k ZL Λ (R,M) (stmtApp f Y)
+      : spill_sound7 k ZL Λ (R,M) (stmtApp f Y)
                      (ann0 (Sp,L, (R', M')::nil))
   | SpillFun
       (ZL : list params)
@@ -81,11 +84,11 @@ Inductive spill_sound (k:nat) :
       (spill_F : (forall n Zs Rf Mf sl_s, get rms n (Rf,Mf)
                          -> get F n Zs
                          -> get sl_F n sl_s
-                         -> spill_sound k ((fst ⊝ F) ++ ZL)
+                         -> spill_sound7 k ((fst ⊝ F) ++ ZL)
                                        (rms ++ Λ) (Rf,Mf) (snd Zs) sl_s
         ))
-      (spill_t : spill_sound k ((fst ⊝ F) ++ ZL) (rms ++ Λ) (R,M) t sl_t)
-      : spill_sound k ZL Λ (R,M) (stmtFun F t)
+      (spill_t : spill_sound7 k ((fst ⊝ F) ++ ZL) (rms ++ Λ) (R,M) t sl_t)
+      : spill_sound7 k ZL Λ (R,M) (stmtFun F t)
                     (annF (Sp,L,rms) sl_F sl_t)
   | SpillLoad
       (ZL : list params)
@@ -96,8 +99,8 @@ Inductive spill_sound (k:nat) :
       (Sp_empty : getSp sl [=] ∅)
       (L_sub : getL sl ⊆ M)
       (card :  cardinal (R \ K ∪ getL sl) <= k)
-      (spill_s : spill_sound k ZL Λ (R \ K ∪ getL sl, M) s (clear_L sl))
-    : spill_sound k ZL Λ (R,M) s sl
+      (spill_s : spill_sound7 k ZL Λ (R \ K ∪ getL sl, M) s (clear_L sl))
+    : spill_sound7 k ZL Λ (R,M) s sl
   | SpillSpill
       (ZL : list params)
       (Λ : list (⦃var⦄ * ⦃var⦄))
@@ -105,8 +108,8 @@ Inductive spill_sound (k:nat) :
       (s : stmt)
       (sl : spilling)
       (Sp_sub : getSp sl ⊆ R)
-      (spill_s : spill_sound k ZL Λ (R, getSp sl ∪ M) s (clear_Sp sl))
-    : spill_sound k ZL Λ (R,M) s sl
+      (spill_s : spill_sound7 k ZL Λ (R, getSp sl ∪ M) s (clear_Sp sl))
+    : spill_sound7 k ZL Λ (R,M) s sl
 .
 
 
@@ -147,7 +150,7 @@ Proof.
       rewrite H3; reflexivity.
 Qed.
 
-Lemma spill_sound_ext'
+Lemma spill_sound7_ext'
       (k : nat)
       (ZL : list params) s
       (Λ Λ2 : list (⦃var⦄ * ⦃var⦄))
@@ -158,7 +161,7 @@ Lemma spill_sound_ext'
     -> R [=] R2
     -> M [=] M2
     -> sl === sl2
-    -> spill_sound k ZL Λ (R,M) s sl -> spill_sound k ZL Λ2 (R2,M2) s sl2
+    -> spill_sound7 k ZL Λ (R,M) s sl -> spill_sound7 k ZL Λ2 (R2,M2) s sl2
 .
 Proof.
   intros Λeq Req Meq sleq H.
@@ -166,13 +169,13 @@ Proof.
   - eapply SpillLet with (Kx:=Kx); simpl; eauto.
     + rewrite <-H2. assumption.
     + rewrite <-H7. assumption.
-    + eapply IHspill_sound; eauto.
+    + eapply IHspill_sound7; eauto.
       rewrite Req. reflexivity.
     + rewrite <- Req. eauto.
     + rewrite <- Req. eauto.
   - econstructor; eauto;
       try rewrite <- H1; try rewrite <- H5; try rewrite <- Req; eauto.
-  - eapply SpillIf; try eapply IHspill_sound1; try eapply IHspill_sound2; eauto;
+  - eapply SpillIf; try eapply IHspill_sound71; try eapply IHspill_sound72; eauto;
       try rewrite <- H4; try rewrite <- H9; try rewrite <- Req; eauto.
   - PIR2_inv.
     eapply SpillApp; eauto;
@@ -196,59 +199,59 @@ Proof.
       * eapply PIR2_app; eauto using list_eq_PIR2.
       * assumption.
       * assumption.
-    + eapply IHspill_sound; eauto.
+    + eapply IHspill_sound7; eauto.
       * eapply PIR2_app; eauto using list_eq_PIR2.
   - eapply SpillLoad; eauto.
     + rewrite <- sleq; eauto.
     + rewrite <- sleq, <- Meq; eauto.
     + rewrite <- Req, <- sleq; eauto.
-    + eapply IHspill_sound; eauto.
+    + eapply IHspill_sound7; eauto.
       * rewrite Req, sleq. reflexivity.
       * rewrite sleq. reflexivity.
   - eapply SpillSpill; eauto.
     + rewrite <- sleq, <- Req; eauto.
-    + eapply IHspill_sound; eauto.
+    + eapply IHspill_sound7; eauto.
       * rewrite Meq, sleq. eauto.
       * rewrite sleq. reflexivity.
 Qed.
 
 
-Instance spill_sound_morph k ZL Λ
-  : Proper (_eq ==> eq ==> @equiv _ _ _ ==> iff) (spill_sound k ZL Λ).
+Instance spill_sound7_morph k ZL Λ
+  : Proper (_eq ==> eq ==> @equiv _ _ _ ==> iff) (spill_sound7 k ZL Λ).
 Proof.
   unfold Proper, respectful; intros; subst; split; intros; inv H.
-  - eapply spill_sound_ext'; eauto; try reflexivity.
+  - eapply spill_sound7_ext'; eauto; try reflexivity.
     eapply H2. eapply H3.
-  - eapply spill_sound_ext'; try eapply H0; try reflexivity.
+  - eapply spill_sound7_ext'; try eapply H0; try reflexivity.
     rewrite H2; eauto. rewrite H3; eauto. symmetry; eauto.
 Qed.
 
-Instance spill_sound_morph_impl k ZL Λ
-  : Proper (_eq ==> eq ==> @equiv _ _ _ ==> impl) (spill_sound k ZL Λ).
+Instance spill_sound7_morph_impl k ZL Λ
+  : Proper (_eq ==> eq ==> @equiv _ _ _ ==> impl) (spill_sound7 k ZL Λ).
 Proof.
   unfold Proper, respectful, impl; intros; subst; intros; inv H.
-  - eapply spill_sound_ext'; try eapply H2; try reflexivity.
+  - eapply spill_sound7_ext'; try eapply H2; try reflexivity.
     rewrite H0; eauto. rewrite H3; eauto. symmetry; eauto.
 Qed.
 
-Instance spill_sound_morph_flip_impl k ZL Λ
-  : Proper (_eq ==> eq ==> @equiv _ _ _ ==> flip impl) (spill_sound k ZL Λ).
+Instance spill_sound7_morph_flip_impl k ZL Λ
+  : Proper (_eq ==> eq ==> @equiv _ _ _ ==> flip impl) (spill_sound7 k ZL Λ).
 Proof.
   unfold Proper, respectful, flip, impl; intros; subst; intros; inv H.
-  - eapply spill_sound_ext'; try eapply H2; try reflexivity.
+  - eapply spill_sound7_ext'; try eapply H2; try reflexivity.
     rewrite H0; eauto. rewrite H3; eauto. symmetry; eauto.
 Qed.
 
-Instance spill_sound_morph' k ZL Λ
-  : Proper (@pe _ _ ==> eq ==> @equiv _ _ _ ==> iff) (spill_sound k ZL Λ).
+Instance spill_sound7_morph' k ZL Λ
+  : Proper (@pe _ _ ==> eq ==> @equiv _ _ _ ==> iff) (spill_sound7 k ZL Λ).
 Proof.
   unfold Proper, respectful; intros; subst; split; intros; inv H.
-  - eapply spill_sound_ext'; eauto; try reflexivity.
-  - eapply spill_sound_ext'; try eapply H0; try reflexivity.
+  - eapply spill_sound7_ext'; eauto; try reflexivity.
+  - eapply spill_sound7_ext'; try eapply H0; try reflexivity.
     rewrite H2; eauto. rewrite H3; eauto. symmetry; eauto.
 Qed.
 
-Lemma spill_sound_spill_sound3
+Lemma spill_sound7_spill_sound
       (k : nat)
       (ZL : list params)
       (Λ : list (⦃var⦄ * ⦃var⦄))
@@ -256,8 +259,8 @@ Lemma spill_sound_spill_sound3
       (s : stmt)
       (sl : spilling)
       (Rsmall: cardinal R <= k)
-  : spill_sound k ZL Λ (R,M) s sl
-    -> SpillSound.spill_sound k ZL Λ (R, M) s sl.
+  : spill_sound7 k ZL Λ (R,M) s sl
+    -> spill_sound k ZL Λ (R, M) s sl.
 Proof.
   intros SPS.
   general induction SPS.
@@ -287,3 +290,23 @@ Proof.
   - eapply spill_sound_load_ext; eauto.
   - eapply spill_sound_spill_ext; eauto.
 Qed.
+
+
+Lemma spill_sound_spill_sound7
+      (k : nat)
+      (ZL : list params)
+      (Λ : list (⦃var⦄ * ⦃var⦄))
+      (R M  : ⦃var⦄)
+      (s : stmt)
+      (sl : spilling)
+  : spill_sound k ZL Λ (R,M) s sl
+    -> spill_sound7 k ZL Λ (R, M) s sl.
+Proof.
+  intros spillSnd.
+  general induction spillSnd; eapply SpillSpill; eauto; eapply SpillLoad; eauto;
+    econstructor; eauto.
+  intros. exploit H4; eauto.
+Qed.
+
+                                                                            
+      
